first attempt at search (and necessary data structure changes)

src/BPlusTree.v
@@ -1,110 +1,407 @@
 From iris.algebra Require Import numbers.
-From iris.heap_lang Require Export proofmode notation lang.
+From iris.heap_lang Require Export proofmode notation.
 From iris.proofmode Require Export proofmode.
-From iris.heap_lang Require Import proofmode.
 From iris.prelude Require Import options.
 
 Section nary_tree.
   Context (A:Set).
+  Context (beq_A : A -> A -> bool).
+  Context (ord_A : A -> A -> Prop).
 
   Inductive nary_tree : Set :=
-  | leaf : list A -> nary_tree
-  | node : list nary_tree -> nary_tree.
+  | leaf (interval : A * A) (l : list A) : nary_tree
+  | node (interval : A * A) (l : list nary_tree) : nary_tree.
+
+  Fixpoint nary_tree_ind'
+    (P : nary_tree -> Prop)
+    (Pleaf : forall interval vals, P (leaf interval vals))
+    (Pnode : forall interval trees, Forall P trees -> P (node interval trees))
+    (t : nary_tree) : P t :=
+    match t with
+    | leaf interval vals => Pleaf interval vals
+    | node interval trees =>
+        Pnode interval trees
+          ((fix nary_tree_ind_aux (l : list nary_tree) : Forall P l :=
+             match l with
+             | [] => Forall_nil_2 P
+             | t :: ts => Forall_cons_2 _ _ _ (nary_tree_ind' P Pleaf Pnode t) (nary_tree_ind_aux ts)
+             end) trees)
+    end.
+
+  Fixpoint nary_tree_wf (t : nary_tree) :=
+    match t with
+    | leaf (low, high) vals => Forall (fun a' => ord_A low a' /\ ord_A a' high) vals
+    | node (low, high) trees =>
+        (fix nary_tree_wf_aux (l : list nary_tree) : Prop :=
+           match l with
+           | [] => True
+           | t :: ts =>
+               nary_tree_wf t /\
+                 match t with
+                 | leaf (low', high') _ => ord_A low low' /\ ord_A high' high
+                 | node (low', high') _ => ord_A low low' /\ ord_A high' high
+                 end /\
+                 nary_tree_wf_aux ts
+           end) trees
+    end.
+
+  Lemma nary_tree_wf_branches interval branches (wf : nary_tree_wf (node interval branches)) :
+    Forall (fun t => nary_tree_wf t) branches.
+  Proof.
+    induction branches.
+    - done.
+    - cbn in wf.
+      destruct interval as [low high].
+      destruct wf as (wf_a & ? & wf_branches).
+      constructor; [done|].
+      apply IHbranches.
+      done.
+  Qed.
+
+  Record Tree : Set :=
+    mkTree {
+        tree : nary_tree;
+        tree_wf : nary_tree_wf tree
+      }.
 
   Fixpoint size (t : nary_tree) : nat :=
     match t with
-    | leaf l => List.length l
-    | node l => list_sum (map size l)
+    | leaf _ l => List.length l
+    | node _ l => list_sum (map size l)
     end.
 
-  Fixpoint In (v : A) (t : nary_tree) {struct t} : Prop :=
+  Fixpoint In_list (v : A) (l : list A) :=
+    match l with
+    | [] => false
+    | x :: xs => orb (beq_A x v) (In_list v xs)
+    end.
+
+  Fixpoint In_tree (v : A) (t : nary_tree) {struct t} : bool :=
     match t with
-    | leaf l => List.In v l
-    | node l => (fix In_list (l : list nary_tree) :=
+    | leaf _ l => In_list v l
+    | node _ l => (fix In_aux (l : list nary_tree) :=
                   match l with
-                  | [] => False
-                  | t :: ts => In v t \/ In_list ts
+                  | [] => false
+                  | t :: ts => orb (In_tree v t) (In_aux ts)
                   end) l
     end.
 End nary_tree.
 
-Section bplus_tree_algos.
-  Definition new_bplus_tree : val :=
-    λ: "_", ref NONEV.
+Section bplus_tree.
+  Definition token_leaf_e v := InjL v.
+  Definition token_branch_e v := InjR v.
+  Definition token_leaf_v v := InjLV v.
+  Definition token_branch_v v := InjRV v.
 
-End bplus_tree_algos.
+  (* Variable tval : Set. *)
+  (* Declare Scope tval_scope. *)
+  (* Delimit Scope tval_scope with t. *)
+  (* Variable teqb : tval -> tval -> bool. *)
+  (* Variable tord : tval -> tval -> Prop. *)
+  (* Notation "v1 < v2" := (tord v1 v2) : tval_scope. *)
+  (* Variable tval_val : tval -> val. *)
+  (* Notation "# v" := (tval_val v) : tval_scope. *)
+  (* Context (tval_dec : forall (v1 v2 : tval), Decision (v1 = v2)). *)
 
-Section bplus_tree_model.
-  Context `{!heapGS Σ}.
-  Notation iProp := (iProp Σ).
+  Definition tval := nat.
+  Variable (ninf pinf : tval).
+  Definition teqb := Nat.eqb.
+  Definition tord := Nat.lt.
+  Axiom pinf_max : forall v, (v < pinf).
+  Axiom ninf_minax : forall v, (ninf < v).
+  Definition tree_spec := Tree tval tord.
 
-  Variable b : nat.
-  Hypothesis beven : Zeven b.
+  Section bplus_tree_model.
+    Context `{!heapGS Σ}.
+    Notation iProp := (iProp Σ).
 
-  Definition tree_spec := nary_tree val.
+    Variable b : nat.
+    Hypothesis beven : Zeven b.
 
-  Fixpoint is_list (hd : val) (xs : list val) : iProp :=
-    match xs with
-    | [] => ⌜hd = NONEV⌝
-    | x :: xs => ∃ (l : loc) hd', ⌜hd = SOMEV #l⌝ ∗ l ↦ (x,hd') ∗ is_list hd' xs
-  end%I.
-
-  Fixpoint is_node (v : val) (t : tree_spec) {struct t} : iProp :=
-    match t with
-    | leaf _ l => ⌜ size _ t < b ⌝ -∗ is_list v l
-    | node _ ts =>
-        ⌜ size _ t >= b ⌝ -∗
-          (∃ (ns : list val),
-              ⌜ b / 2 <= length ns <= b ⌝ ∗
-              ⌜ length ns = length ts ⌝ ∗
-              is_list v ns ∗
-              ((fix is_internal_node_list (ns : list val) (ts : list tree_spec) {struct ts} : iProp :=
-                  match ns, ts with
-                  | [], [] => True
-                  | n :: ns, t :: ts => is_node n t ∗ is_internal_node_list ns ts
-                  | _, _ => False
-                end)
-                 ns ts))
+    Fixpoint is_list (hd : val) (xs : list val) : iProp :=
+      match xs with
+      | [] => ⌜hd = NONEV⌝
+      | x :: xs => ∃ (l : loc) hd', ⌜hd = SOMEV #l⌝ ∗ l ↦ (x, hd') ∗ is_list hd' xs
     end%I.
 
-  Definition is_root_node (v : val) (t : tree_spec) : iProp :=
-    match t with
-    | leaf _ l => ⌜ size _ t < b ⌝ -∗ is_list v l
-    | node _ ts =>
-        ⌜ size _ t >= b ⌝ -∗
-          (∃ ns : list val,
-              ⌜ 2 <= length ns <= b ⌝ ∗
-              is_list v ns ∗
-              ((fix is_branching_root_node_list (ns : list val) (ts : list tree_spec) :=
-                 match ns, ts with
-                 | [], [] => True
-                 | n :: ns, t :: ts => is_node n t ∗ is_branching_root_node_list ns ts
-                 | _, _ => False
-                 end)
-                 ns ts))
-    end%I.
+    Definition leaf_node v (t : tree_spec) (interval : tval * tval) (vals : list tval) :=
+      let (low, high) := interval in
+      (∃ (ptr : loc) (lhd : val), ⌜ size _ (tree _ _ t) < b ⌝ ∗ ⌜ v = token_leaf_v #ptr ⌝ ∗ ptr ↦ ((#low, #high), lhd) ∗ is_list lhd (map (fun (x : tval) => #x) vals))%I.
 
-  Definition is_bplus_tree (v : val) (t : tree_spec) : iProp :=
-    (∃ (l : loc) (r : val), ⌜v = #l⌝ ∗ l ↦ r ∗ is_root_node r t)%I.
+    Definition branch_node v (t : nary_tree tval) (* (t_wf : nary_tree_wf _ tord t) *) (interval : tval * tval) ts node_size_min (is_node : forall (_ : val) (t : nary_tree tval), nary_tree_wf _ _ t -> iProp) :=
+      let (low, high) := interval in
+      (∃ (ptr : loc) l (ns : list val),
+          (* these two should be moved to spec *)
+          ⌜ size _ t >= b ⌝ ∗
+          ⌜ node_size_min <= length ns <= b ⌝ ∗
+          (* the rest are fine ? *)
+          ⌜ v = token_branch_v #ptr ⌝ ∗
+          ⌜ length ns = length ts ⌝ ∗
+          ptr ↦ (((#low), (#high)), l) ∗
+          is_list l ns ∗
+          ((fix branch_node_list (ns : list val) (ts : list tree_spec) {struct ts} : iProp :=
+              match ns, ts with
+              | [], [] => True
+              | n :: ns, t :: ts => is_node n (tree _ _ t) (tree_wf _ _ t) ∗ branch_node_list ns ts
+              | _, _ => False
+              end)
+             ns ts))%I.
 
-End bplus_tree_model.
+    Fixpoint is_node (v : val) (t : nary_tree tval) (t_wf : nary_tree_wf _ _ t) {struct t} : iProp :=
+      match t as t0 return t = t0 -> iProp with
+      | leaf _ interval l => fun _ => leaf_node v {| tree := t; tree_wf := t_wf |} interval l
+      | node _ interval ts => fun t_t0 =>
+          let t_wf' := nary_tree_wf_branches
+                         tval
+                         tord
+                         interval
+                         ts
+                         (eq_rect
+                            t
+                            _
+                            t_wf
+                            (node _ interval ts)
+                            t_t0) in
+          let trees := ((fix is_node_list (ts : list (nary_tree tval)) (ts_wf : Forall (fun t => nary_tree_wf _ _ t) ts) : list tree_spec :=
+              match ts as ts0 return ts = ts0 -> list tree_spec with
+              | [] => fun _ => []
+              | t' :: ts' =>
+                  fun ts_ts0 =>
+                    let ts_wf_cons := Forall_cons_1
+                                        (fun x => nary_tree_wf _ _ x)
+                                        t'
+                                        ts'
+                                        (eq_rect ts _ ts_wf (t' :: ts') ts_ts0) in
+                    let t'_wf := proj1 ts_wf_cons in
+                    let ts'_wf := proj2 ts_wf_cons in
+                    {| tree := t'; tree_wf := t'_wf |} :: is_node_list ts' ts'_wf
+              end eq_refl) ts t_wf') in
+          branch_node v t interval trees (b / 2) is_node
+      end eq_refl%I.
 
-Section bplus_tree_proofs.
-  Context `{!heapGS Σ}.
-  Notation iProp := (iProp Σ).
+    Definition is_bplus_tree (v : val) (t : tree_spec) (* (t_wf : nary_tree_wf _ tord t) *) : iProp :=
+      match t with
+      | leaf _ interval l => leaf_node v t interval l
+      | node _ interval ts => branch_node v t interval ts 2 is_node
+      end%I.
 
-  Variable b : nat.
-  Hypothesis beven : Zeven b.
+  End bplus_tree_model.
 
-  Theorem new_bplus_tree_spec:
-    {{{ True }}} new_bplus_tree #() {{{ v, RET v; is_bplus_tree b v (leaf val []) }}}.
-  Proof.
-    iIntros (Φ) "_ HPost".
-    wp_lam; wp_alloc v.
-    iApply "HPost".
-    iExists v, NONEV.
-    iFrame.
-    done.
-  Qed.
+  Section bplus_tree_algos.
+    Definition new_bplus_tree : val :=
+      λ: "_",
+        let: "ptr" := ref ((#ninf, #pinf), NONEV) in
+        token_leaf_e "ptr".
 
-End bplus_tree_proofs.
+    Definition search_list : val :=
+      rec: "search_list" "arg" :=
+        let: "p" := Fst "arg" in
+        let: "target" := Snd "arg" in
+        match: "p" with
+          NONE => #false
+        | SOME "l" =>
+            let: "val" := Fst !"l" in
+            if: "val" = "target"
+            then #true
+            else "search_list" (Snd !"l", "target")
+        end.
+
+    Definition search_bplus_tree : val :=
+      rec: "search_bplus_tree" "arg" :=
+        let: "t" := Fst "arg" in
+        let: "target" := Snd "arg" in
+        match: "t" with
+          InjL "ptr" =>
+            let: "lhd" := Snd !"ptr" in
+            search_list ("lhd", "target")
+        | InjR "ptr" =>
+            let: "lhd" := Snd !"ptr" in
+            let: "f" :=
+            rec: "search_node_list" "arg" :=
+              let: "p" := Fst "arg" in
+              let: "target" := Snd "arg" in
+              match: "p" with
+                NONE => #false
+              | SOME "l" =>
+                  let: "val" := Fst !"l" in
+                  match: "val" with
+                    InjL "ptr" =>
+                      let: "interval" := Fst !"ptr" in
+                      let: "low" := Fst "interval" in
+                      let: "high" := Snd "interval" in
+                      if: (BinOp LeOp "low" "target") && (BinOp LeOp "target" "high")
+                      then "search_bplus_tree" ("val", "target")
+                      else "search_node_list" (Snd !"l", "target")
+                  | InjR "ptr" =>
+                      let: "interval" := Fst !"ptr" in
+                      let: "low" := Fst "interval" in
+                      let: "high" := Snd "interval" in
+                      if: (BinOp LeOp "low" "target") && (BinOp LeOp "target" "high")
+                      then "search_bplus_tree" ("val", "target")
+                      else "search_node_list" (Snd !"l", "target")
+                  end
+              end in
+              "f" ("lhd", "target")
+        end%E.
+
+  End bplus_tree_algos.
+
+  Section bplus_tree_proofs.
+    Context `{!heapGS Σ}.
+    Notation iProp := (iProp Σ).
+
+    Variable b : nat.
+    Hypothesis beven : Zeven b.
+    Hypothesis bpos : 0 < b.
+
+    Definition empty_tree := leaf tval (ninf, pinf) [].
+    Lemma empty_tree_wf : nary_tree_wf _ tord empty_tree.
+    Proof. apply Forall_nil_2. Qed.
+
+    Theorem new_bplus_tree_spec:
+      {{{ True }}} new_bplus_tree #() {{{ v, RET v; is_bplus_tree b v empty_tree (* empty_tree_wf *) }}}.
+    Proof using bpos.
+      iIntros (Φ) "_ HPost".
+      wp_lam; wp_alloc ptr; wp_pures.
+      iApply "HPost".
+      iExists ptr, NONEV.
+      iSplitR; [done|].
+      iSplitR; [done|].
+      iSplitL; [done|].
+      done.
+    Qed.
+
+    Lemma tree_leaf_token_leaf v low high l (* (wf : (nary_tree_wf _ _ (leaf _ (low, high) l))) *):
+      is_bplus_tree b v (leaf _ (low, high) l) (* wf *) ⊢ ∃ x, ⌜ v = token_leaf_v x ⌝.
+    Proof.
+      iIntros "Hv".
+      iDestruct "Hv" as (? ?) "[% [% Hv]]".
+      iExists #ptr.
+      done.
+    Qed.
+
+    Lemma tree_node_token_branch v low high l (* (wf : nary_tree_wf _ _ (node _ (low, high) l)) *):
+      is_bplus_tree b v (node _ (low, high) l) (* wf *) ⊢ ∃ x, ⌜ v = token_branch_v x ⌝.
+    Proof.
+      iIntros "Hv".
+      iDestruct "Hv" as (? ? ? ?) "(_ & ? & _)".
+      iExists #ptr.
+      done.
+    Qed.
+
+    Lemma bool_decide_true_eqb (x y : nat) :
+      bool_decide (#x = #y) = true -> Nat.eqb x y = true.
+    Proof.
+      clear bpos.
+      intro.
+      apply bool_decide_eq_true_1 in H.
+      injection H as H.
+      assert (x = y) by lia; subst.
+      rewrite Nat.eqb_refl.
+      done.
+    Qed.
+
+    Lemma bool_decide_false_eqb (x y : nat) :
+      bool_decide (#x = #y) = false -> Nat.eqb x y = false.
+    Proof.
+      clear bpos.
+      intro.
+      apply bool_decide_eq_false in H.
+      assert (not (Z.of_nat x = Z.of_nat y)) by congruence.
+      assert (not (x = y)) by auto.
+      apply Nat.eqb_neq in H1.
+      done.
+    Qed.
+
+    Lemma search_list_spec (v : val) (l : list tval) (target : tval):
+      {{{ is_list v (map (fun (x : tval) => (#x)) l) }}} search_list (v, (#target))%V {{{ r, RET r; ⌜ r = #(In_list _ teqb target l) ⌝ ∗ is_list v (map (fun (x : tval) => (#x)) l) }}}.
+    Proof.
+      clear bpos.
+      iIntros (Φ) "Hl HPost".
+      iInduction l as [|x l] "IH" forall (Φ v); wp_rec; wp_pures.
+      - iDestruct "Hl" as "->".
+        wp_match.
+        iApply "HPost".
+        iSplitL; [|done].
+        iPureIntro.
+        done.
+      - iDestruct "Hl" as (l' ?) "(-> & Hl' & Hl)".
+        wp_match; wp_load; wp_pures.
+        destruct (bool_decide (#x = #target)) eqn:?.
+        + wp_pures.
+          iApply "HPost".
+          iSplitR "Hl' Hl".
+          2:(iExists l', hd'; iFrame; done).
+          iPureIntro.
+          cbn; unfold teqb.
+          rewrite (bool_decide_true_eqb _ _ Heqb0).
+          done.
+        + wp_pures; wp_load; wp_pures.
+          iApply ("IH" $! Φ hd' with "Hl").
+          iNext.
+          iIntros (?) "[% Hl]".
+          iApply "HPost".
+          iClear "IH".
+          iSplitR.
+          * iPureIntro.
+            unfold In_list, teqb.
+            rewrite (bool_decide_false_eqb _ _ Heqb0).
+            cbn.
+            done.
+          * iExists l', hd'.
+            iFrame.
+            done.
+    Qed.
+
+    Theorem search_bplus_tree_spec (t : tree_spec) (* (wf : nary_tree_wf _ _ t) *) (v : val) (target : nat) :
+      {{{ is_bplus_tree b v t (* wf *) }}} search_bplus_tree (v, #target)%V {{{ r, RET r; ⌜ r = #(In_tree _ teqb target t) ⌝ ∗ is_bplus_tree b v t (* wf *) }}}.
+    Proof using bpos.
+      iIntros (Φ) "Hv HPost".
+      iLöb as "IH" forall (v t).
+      
+      destruct t as [(low & high)|(low & high) ts].
+      - iPoseProof (tree_leaf_token_leaf with "Hv") as (?) "->".
+        iDestruct "Hv" as (? ?) "(% & % & Hptr & Hlhd)".
+        assert (x = #ptr) by (unfold token_leaf_v in H0; congruence); subst.
+        wp_rec; wp_load; wp_pures.
+        iApply (search_list_spec with "Hlhd").
+        iNext.
+        iIntros (?) "[% Hlhd]".
+        iApply "HPost".
+        iSplitR; [done|].
+        iExists ptr, lhd.
+        iFrame.
+        done.
+
+      - iPoseProof (tree_node_token_branch with "Hv") as (?) "->".
+        iDestruct "Hv" as (ptr lhd ns) "(% & % & % & % & Hptr & Hlhd & Hns)".
+        assert (x = #ptr) by (unfold token_branch_v in H1; congruence); subst.
+        iInduction ns as [|nhd nrest] "IH'"; [rewrite nil_length in H0; lia|].
+        destruct ts as [|thd trest]; [rewrite nil_length in H2; lia|].
+        iDestruct "Hlhd" as (l0 ?) "(-> & Hl0 & Hnrest)".
+        iDestruct "Hns" as "[Hthd Htrest]".
+        destruct thd.
+        + destruct interval as [low' high'].
+          iDestruct "Hthd" as (ptr' leaves) "(% & -> & Hptr' & Hleaves)".
+          wp_rec; wp_load; wp_load; wp_load; wp_pures.
+          destruct (bool_decide (Z.le (Z.of_nat low') (Z.of_nat target))) eqn:?; wp_pures.
+          * destruct (bool_decide (Z.le (Z.of_nat target) (Z.of_nat high'))) eqn:?; wp_pures.
+            -- iClear "IH'".
+               iApply ("IH" $! (token_leaf_v #ptr') (leaf _ (low', high') l) with "[Hptr' Hleaves]").
+               { iExists ptr', leaves.
+                 iSplitR; [done|].
+                  iSplitR; [done|].
+                  iSplitL "Hptr'"; [done|].
+                  done. }
+                iNext.
+                iIntros (?) "[% Htree]".
+                iApply "HPost".
+                iSplitR.
+                { iPureIntro.
+                  cbn in *.
+                  
+                
+    Qed.
+
+  End bplus_tree_proofs.
+End bplus_tree.
